

1 LayerNorm Backward Derivation for One Row

1.1 Forward Pass

For input $\mathbf{x} \in \mathbb{R}^{1 \times N}$, LayerNorm computes:

$$\mu = \frac{1}{N} \sum_{i=1}^N x_i \quad (1)$$

$$\sigma^2 = \frac{1}{N} \sum_{i=1}^N (x_i - \mu)^2 \quad (2)$$

$$\hat{x}_i = \frac{x_i - \mu}{\sqrt{\sigma^2 + \epsilon}} \quad (3)$$

$$y_i = \gamma \hat{x}_i + \beta \quad (4)$$

For simplicity, let's assume $\gamma = 1$ and $\beta = 0$ (they can be added back easily), so:

$$y_i = \frac{x_i - \mu}{\sqrt{\sigma^2 + \epsilon}} \quad (5)$$

1.2 Jacobian Derivation

We need to compute $\frac{\partial y_i}{\partial x_j}$ for all $i, j \in \{1, 2, \dots, N\}$.

Let $\sigma = \sqrt{\sigma^2 + \epsilon}$ for notation simplicity.

$$\frac{\partial y_i}{\partial x_j} = \frac{\partial}{\partial x_j} \left(\frac{x_i - \mu}{\sigma} \right) \quad (6)$$

Using the quotient rule and chain rule:

$$\frac{\partial y_i}{\partial x_j} = \frac{1}{\sigma} \frac{\partial (x_i - \mu)}{\partial x_j} - \frac{x_i - \mu}{\sigma^2} \frac{\partial \sigma}{\partial x_j} \quad (7)$$

1.2.1 Computing $\frac{\partial \mu}{\partial x_j}$

$$\frac{\partial \mu}{\partial x_j} = \frac{\partial}{\partial x_j} \left(\frac{1}{N} \sum_{k=1}^N x_k \right) = \frac{1}{N} \quad (8)$$

1.2.2 Computing $\frac{\partial \sigma}{\partial x_j}$

$$\frac{\partial \sigma}{\partial x_j} = \frac{\partial}{\partial x_j} \sqrt{\sigma^2 + \epsilon} = \frac{1}{2\sigma} \frac{\partial \sigma^2}{\partial x_j} \quad (9)$$

$$\frac{\partial \sigma^2}{\partial x_j} = \frac{\partial}{\partial x_j} \left(\frac{1}{N} \sum_{k=1}^N (x_k - \mu)^2 \right) \quad (10)$$

$$= \frac{1}{N} \sum_{k=1}^N 2(x_k - \mu) \left(\delta_{kj} - \frac{1}{N} \right) \quad (11)$$

$$= \frac{2}{N} (x_j - \mu) - \frac{2}{N^2} \sum_{k=1}^N (x_k - \mu) \quad (12)$$

Since $\sum_{k=1}^N (x_k - \mu) = 0$:

$$\frac{\partial \sigma^2}{\partial x_j} = \frac{2}{N} (x_j - \mu) \quad (13)$$

Therefore:

$$\frac{\partial \sigma}{\partial x_j} = \frac{1}{2\sigma} * \frac{2}{N} (x_j - \mu) = \frac{x_j - \mu}{N\sigma} \quad (14)$$

1.2.3 Combining terms

$$J_{ij} = \frac{\partial y_i}{\partial x_j} = \frac{1}{\sigma} \left(\delta_{ij} - \frac{1}{N} \right) - \frac{x_i - \mu}{\sigma^2} * \frac{x_j - \mu}{N\sigma} \quad (15)$$

$$= \frac{1}{\sigma} \left(\delta_{ij} - \frac{1}{N} \right) - \frac{(x_i - \mu)(x_j - \mu)}{N\sigma^3} \quad (16)$$

$$= \frac{1}{\sigma} \left(\delta_{ij} - \frac{1}{N} - \frac{\hat{x}_i \hat{x}_j}{N} \right) \quad (17)$$

where $\hat{x}_i = \frac{x_i - \mu}{\sigma}$.

1.3 Jacobian Matrix

$$J_{(N \times N)} = \frac{\partial y}{\partial x} = \frac{1}{\sigma} \left(I - \frac{1}{N} \mathbf{1}^T \mathbf{1} - \frac{\hat{x}^T \hat{x}}{N} \right) \quad (18)$$

- $\mathbf{1}$ is a row vector with all elements equal to 1 and the same shape as \mathbf{x} .

1.4 Backward Pass

Given $\frac{\partial L}{\partial \mathbf{y}} = \mathbf{dy} \in \mathbb{R}^{1 \times N}$, we compute:

$$dx = dy \cdot J \quad (19)$$

$$= \frac{1}{\sigma} \left(dy - \frac{1}{N} \underbrace{(dy \cdot \mathbf{1}^T)}_{\text{scalar1}} \mathbf{1} - \frac{1}{N} \underbrace{(dy \cdot \hat{x}^T)}_{\text{scalar2}} \hat{x} \right) \quad (20)$$

$$= \frac{1}{\sigma} (dy - \text{mean}(dy) \mathbf{1} - \text{mean}(dy \odot \hat{x}) \hat{x}) \quad (21)$$

$$(22)$$

Let:

- $\text{mean}(\mathbf{dy}) = \frac{1}{N} \sum_{i=1}^N dy_i$
- $\text{mean}(\mathbf{dy} \odot \hat{\mathbf{x}}) = \frac{1}{N} \sum_{i=1}^N dy_i \hat{x}_i$

where $\sigma = \sqrt{\frac{1}{N} \sum_{i=1}^N (x_i - \mu)^2 + \epsilon}$ and $\hat{\mathbf{x}} = \frac{\mathbf{x} - \mu}{\sigma}$.

1.5 Backward Pass add in w

$$dx = (w \odot dy) \cdot J \quad (23)$$

$$= \frac{1}{\sigma} \left((w \odot dy) - \frac{1}{N} \underbrace{((w \odot dy) \cdot \mathbf{1}^T)}_{\text{scalar1}} \mathbf{1} - \frac{1}{N} \underbrace{((w \odot dy) \cdot \hat{x}^T)}_{\text{scalar2}} \hat{x} \right) \quad (24)$$

$$= \frac{1}{\sigma} ((w \odot dy) - \text{mean}((w \odot dy)) \mathbf{1} - \text{mean}((w \odot dy) \odot \hat{x}) \hat{x}) \quad (25)$$

$$(26)$$